Extended Lbls , mostly extended Procstep - need to define x(disp) and x(dup) rules and replacement syntax and how it works.

PiLL/PiLL/Definitions.lean
@@ -170,12 +170,12 @@ notation:80 x "⟦𝐋⟧." P:80 => Proc.selectL x P
 notation:80 x "⟦𝐑⟧." P:80 => Proc.selectR x P
 notation:80 "⸨" x "⸩.case⦃𝐋" " : " P:80 ", " "𝐑" " : " Q :80"⦄" => Proc.offer x P Q
 notation:80 x "⟦" A "⟧:" P => Proc.output x P A
-notation:80 x "⸨" A "⸩:" P => Proc.input x P A
+notation:80 x "⸨" X "⸩:" P => Proc.input x P X
 notation:80 "!" x ".⦃" P "⦄" => Proc.server x P
 notation:80 x "⟦USE⟧." P => Proc.consume x P
 notation:80 x "⟦DUP⟧⸨" y "⸩." P => Proc.duplicate x y P
 notation:80 x "⟦DISP⟧." P => Proc.dispose x P
-notation:80 x "⟷" y => Proc.link x y
+notation:80 x "⟷ₚ" y => Proc.link x y
 
 notation "𝟘" => Proc.nil
 infixr:65 " |ₚ " => Proc.par
@@ -472,11 +472,6 @@ theorem AlphaEq.comm (P Q : Proc) : (P =ₐ Q) = (Q =ₐ P) := by
   · apply AlphaEq.symm
   · apply AlphaEq.symm
 
-
-
-
-
-
 -- lemma renameBound_comm {x y a b : PName} {P : Proc} :
 --   (hxy : x ≠ y) → (hab : a ≠ b) → (hxb : x ≠ b) → (hya : y ≠ a) →
 --   renameBound x a (renameBound y b P) = renameBound y b (renameBound x a P) := by
@@ -559,663 +554,707 @@ theorem AlphaEq.comm (P Q : Proc) : (P =ₐ Q) = (Q =ₐ P) := by
 --   (h : renameBound y w1 P =ₐ renameBound y' w1 Q) :
 --   (renameBound y w2 P =ₐ renameBound y' w2 Q) := by sorry
 
+theorem AlphaEq.trans (P Q R : Proc) (hPQ : P =ₐ Q) (hQR : Q =ₐ R) : P =ₐ R := by sorry
+--   induction P.size + Q.size using Nat.strong_induction_on generalizing P Q R
+--   rename_i n ih
+--   cases hPQ <;> cases hQR
+--   case nil.nil => rfl
+--   case par.par =>
+--     rename_i P1 Q1 P2 Q2 h1 h2 Q1' Q2' h5 h6
+--     apply AlphaEq.par
+--     · sorry
 
 
+--------------------------------------- ENVIRONMENTS ---------------------------------------
 
+abbrev Env := Finset (PName × Types)
 
+abbrev EmptyEnv : Env := ∅
 
+/- FIXME: eval does not work since non-computable -/
+noncomputable instance : Repr Env where
+  reprPrec (Γ : Env) _ :=
+    if Γ = ∅ then "∅"
+    else
+      let entries := Γ.toList.map (fun (x, A) => s!"{x} ∶ {reprStr A}")
+      String.intercalate "‚ " entries
 
+noncomputable instance : ToString Env where
+  toString e := reprStr e
 
+def Env.mk (x : PName) (A : Types) : Env :=
+  {(x, A)}
 
+infixr:90 " ∶ " => Env.mk
 
+def Env.linear (Δ : Env) : Prop :=
+  (Δ.image Prod.fst).card = Δ.card
 
+def Env.names (Δ : Env) : Finset (PName) :=
+  (Δ.image Prod.fst)
 
+def Env.disjoint (Δ Γ : Env) : Prop :=
+  (Δ.image Prod.fst ∩ Γ.image Prod.fst).card = 0
 
+noncomputable def Env.lookup (Δ : Env) (x : PName) : Option Types :=
+  -- Finset.fold (· ∪ ·) none (fun p => if p.fst = x then p.snd else none) Δ
+  (Δ.toList.find? (fun p => p.fst = x)).map Prod.snd
 
-theorem AlphaEq.trans (P Q R : Proc) (hPQ : P =ₐ Q) (hQR : Q =ₐ R) : P =ₐ R := by
-  induction P.size + Q.size using Nat.strong_induction_on generalizing P Q R
-  rename_i n ih
-  cases hPQ <;> cases hQR
-  case nil.nil => rfl
-  case par.par =>
-    rename_i P1 Q1 P2 Q2 h1 h2 Q1' Q2' h5 h6
-    apply AlphaEq.par
-    · sorry
+notation Δ "⸨" x "⸩ₑ" => Env.lookup Δ x
 
+-- Order independent equality for environments
+@[simp]
+def Env.Eq (Δ Γ : Env) : Prop :=
+  ∀ x : (PName), Δ⸨x⸩ₑ = Γ⸨x⸩ₑ
 
+notation Δ " =ₑ " Γ => Env.Eq Δ Γ
 
+-- Eq reflexivity
+@[simp]
+theorem Env.Eq_refl (Δ : Env) : Δ =ₑ Δ :=
+  fun _ => rfl
 
+-- Eq symmetry
+@[simp]
+theorem Env.Eq_symm (Δ Γ : Env) (h : Δ =ₑ Γ) : Γ =ₑ Δ :=
+  fun x => (h x).symm
 
+-- Eq transitivity
+@[simp]
+theorem Env.Eq_trans (Δ Γ Ε : Env) (h₁ : Δ =ₑ Γ) (h₂ : Γ =ₑ Ε) : Δ =ₑ Ε :=
+  fun x => Eq.trans (h₁ x) (h₂ x)
+
+instance : Equivalence Env.Eq :=
+⟨Env.Eq_refl, @Env.Eq_symm, @Env.Eq_trans⟩
 
+@[simp]
+def Env.merge (Δ Γ : Env) : Env := Δ ∪ Γ
 
+infixl:85 "‚ " => Env.merge
 
-
-
-
-
-
-
-
-
-
-
-
-
-
-
-
-
-
-
-
-
-
-
-
-
-
-
-
-
-
-
-
-
-
-
-
-
-
-
-
-
-
-
-
-
-
--- --------------------------------------- ENVIRONMENTS ---------------------------------------
-
--- abbrev Env := Finset (PName × Types)
-
--- abbrev EmptyEnv : Env := ∅
-
--- /- FIXME: eval does not work since non-computable -/
--- noncomputable instance : Repr Env where
---   reprPrec (Γ : Env) _ :=
---     if Γ = ∅ then "∅"
---     else
---       let entries := Γ.toList.map (fun (x, A) => s!"{x} ∶ {reprStr A}")
---       String.intercalate "‚ " entries
-
--- noncomputable instance : ToString Env where
---   toString e := reprStr e
-
--- def Env.mk (x : PName) (A : Types) : Env :=
---   {(x, A)}
-
--- infixr:90 " ∶ " => Env.mk
-
--- def Env.linear (Δ : Env) : Prop :=
---   (Δ.image Prod.fst).card = Δ.card
-
--- def Env.names (Δ : Env) : Finset (PName) :=
---   (Δ.image Prod.fst)
-
--- def Env.disjoint (Δ Γ : Env) : Prop :=
---   (Δ.image Prod.fst ∩ Γ.image Prod.fst).card = 0
-
--- noncomputable def Env.lookup (Δ : Env) (x : PName) : Option Types :=
---   -- Finset.fold (· ∪ ·) none (fun p => if p.fst = x then p.snd else none) Δ
---   (Δ.toList.find? (fun p => p.fst = x)).map Prod.snd
-
--- notation Δ "⸨" x "⸩ₑ" => Env.lookup Δ x
-
--- -- Order independent equality for environments
--- @[simp]
--- def Env.Eq (Δ Γ : Env) : Prop :=
---   ∀ x : (PName), Δ⸨x⸩ₑ = Γ⸨x⸩ₑ
-
--- notation Δ " =ₑ " Γ => Env.Eq Δ Γ
-
--- -- Eq reflexivity
--- @[simp]
--- theorem Env.Eq_refl (Δ : Env) : Δ =ₑ Δ :=
---   fun _ => rfl
-
--- -- Eq symmetry
--- @[simp]
--- theorem Env.Eq_symm (Δ Γ : Env) (h : Δ =ₑ Γ) : Γ =ₑ Δ :=
---   fun x => (h x).symm
-
--- -- Eq transitivity
--- @[simp]
--- theorem Env.Eq_trans (Δ Γ Ε : Env) (h₁ : Δ =ₑ Γ) (h₂ : Γ =ₑ Ε) : Δ =ₑ Ε :=
---   fun x => Eq.trans (h₁ x) (h₂ x)
-
--- instance : Equivalence Env.Eq :=
--- ⟨Env.Eq_refl, @Env.Eq_symm, @Env.Eq_trans⟩
-
--- @[simp]
--- def Env.merge (Δ Γ : Env) : Env := Δ ∪ Γ
-
--- infixl:85 "‚ " => Env.merge
-
--- -- Merge identity
--- @[simp]
--- theorem Env.merge_unitR (Δ : Env) : Δ‚ ∅ = Δ := by
---   simp
-
--- @[simp]
--- theorem Env.merge_unitL (Δ : Env) : ∅‚ Δ = Δ := by
---   simp
-
--- -- Merge commutivity
--- -- theorem mergeEnv.comm (Δ Γ : Env) : disjointEnv Δ Γ → mergeEnv Δ Γ = mergeEnv Γ Δ := by
--- @[simp]
--- theorem Env.merge_comm (Δ Γ : Env) : Δ‚ Γ = Γ‚ Δ := by
---   simp [Finset.union_comm]
-
--- -- Merge associativity
--- @[simp]
--- theorem Env.merge_assoc (Δ Γ Ε : Env) : Δ‚ Γ‚ Ε = Δ‚ (Γ‚ Ε) := by
---   simp
-
--- @[simp]
--- lemma Env.merge_swap_last (Γ Δ Ξ : Env) :
---   (Γ‚ Δ)‚ Ξ = (Γ‚ Ξ)‚ Δ := by
---   rw [Env.merge_comm, ←Env.merge_assoc]
---   conv => lhs ; lhs ; rw [Env.merge_comm]
-
--- @[simp]
--- lemma Env.merge_move_last_two_left (Γ Δ Ξ Ε : Env) :
---   Γ‚ Δ‚ Ξ‚ Ε = Γ‚ Ε‚ Δ‚ Ξ := by
---   rw [Env.merge_swap_last, Env.merge_swap_last Γ Δ Ε]
-
--- @[simp]
--- lemma Env.merge_move_second_two_right (Γ Δ Ξ Ε : Env) :
---   Γ‚ Δ‚ Ξ‚ Ε = Γ‚ Ξ‚ Ε‚ Δ := by
---   rw [Env.merge_swap_last Γ Δ Ξ, Env.merge_swap_last]
-
-
--- ------------------------------------ HYPER-ENVIRONMENTS ------------------------------------
-
--- abbrev HyperEnv := Finset (Env)
-
--- abbrev EmptyHyperEnv : HyperEnv := ∅
-
--- instance : Coe Env HyperEnv := ⟨fun Γ => ({Γ} : HyperEnv)⟩
-
--- /- FIXME: eval does not work since non-computable -/
--- open Lean in
--- noncomputable instance : Repr HyperEnv where
---   reprPrec (𝒢 : HyperEnv) _ :=
---     if 𝒢 = ∅ then "∅"
---     else
---       let entries := 𝒢.toList.map repr
---       Format.joinSep entries " |ₕ "
-
--- noncomputable instance : ToString HyperEnv where
---   toString g := reprStr g
-
--- def pairwise {α : Type} (r : α → α → Prop) (s : Finset α) : Prop :=
---   ∀ x ∈ s, ∀ y ∈ s, y ≠ x → r x y
-
--- def HyperEnv.linear (𝒢 : HyperEnv) : Prop :=
---   ∀ Δ ∈ 𝒢, Δ.linear ∧                               -- ensure each env is linear
---   pairwise (fun Δ Γ => Δ.disjoint Γ) 𝒢              -- ensure pairwise env disjointness
-
--- def HyperEnv.names (𝒢 : HyperEnv) : Finset PName :=
---   Finset.fold (· ∪ ·) ∅ Env.names 𝒢
-
--- -- Lookup method for finding the type of a name in the hyperenvironment
--- noncomputable def HyperEnv.lookup (𝒢 : HyperEnv) (x : PName) : Option Types :=
---   (𝒢.toList.find? (fun Δ => Δ⸨x⸩ₑ ≠ none)) >>= fun Δ  => Δ⸨x⸩ₑ
-
--- notation:60 𝒢 "⸨" x "⸩ₕ" => HyperEnv.lookup 𝒢 x
-
--- def HyperEnv.disjoint (𝒢 ℋ : HyperEnv) : Prop :=
---   -- 1. ensure both hyperenvs are lienar
---   -- 2. ensure disjoint env names
---   -- 3. ensure no duplicate definitions across hyperenvs
---     -- s.t. an unambigous lookup in the individual hyperenvs
---     -- yields an unambigous lookupin the merged hyperenv
---     -- i.e. the intersection of their defined names is empty
---   𝒢.linear ∧ ℋ.linear ∧
---   (𝒢 ∩ ℋ).card = 0 ∧
---   (𝒢.names ∩ ℋ.names).card = 0
-
--- -- Order independent equality for hyper-environments
--- @[simp]
--- def HyperEnv.Eq (𝒢 ℋ : HyperEnv) : Prop :=
---   -- (1) 𝒢 and ℋ must define the same names
---   -- (2) The typing of all defined names must match i.e. ∀ x, 𝒢(x) = ℋ(x)
---   HyperEnv.names 𝒢 = HyperEnv.names ℋ ∧
---   ∀ x ∈ HyperEnv.names 𝒢, 𝒢⸨x⸩ₕ = ℋ⸨x⸩ₕ
-
--- notation 𝒢 " =ₕ " ℋ => HyperEnv.Eq 𝒢 ℋ
-
--- -- Eq reflexivity
--- @[simp]
--- theorem HyperEnv.Eq_refl (𝒢 : HyperEnv) : 𝒢 =ₕ 𝒢 := by
---   simp
-
--- -- Eq symmetry
--- @[simp]
--- theorem HyperEnv.Eq_symm (𝒢 ℋ : HyperEnv) (h : 𝒢 =ₕ ℋ) : ℋ =ₕ 𝒢 := by
---   rcases h with ⟨h_names, h_vals⟩
---   refine ⟨h_names.symm, ?vals⟩
---   intro x hx
---   rw [h_names] at h_vals
---   apply (h_vals x hx).symm
-
--- -- Eq transitivity
--- @[simp]
--- theorem HyperEnv.Eq_trans (𝒢 ℋ 𝒦 : HyperEnv) (h₁ : 𝒢 =ₕ ℋ) (h₂ : ℋ =ₕ 𝒦) :
---   𝒢 =ₕ 𝒦 := by
---   rcases h₁ with ⟨h₁_names, h₁_vals⟩
---   rcases h₂ with ⟨h₂_names, h₂_vals⟩
---   refine ⟨?names, ?vals⟩
---   · rw [h₁_names, h₂_names]
---   · intro x hx
---     have hxH : x ∈ ℋ.names := by rw [← h₁_names]; exact hx
---     calc
---       𝒢⸨x⸩ₕ = ℋ⸨x⸩ₕ := h₁_vals x hx
---       _          = 𝒦⸨x⸩ₕ := h₂_vals x hxH
-
--- instance : Equivalence HyperEnv.Eq :=
--- ⟨HyperEnv.Eq_refl, @HyperEnv.Eq_symm, @HyperEnv.Eq_trans⟩
-
--- @[simp]
--- abbrev HyperEnv.merge (𝒢 ℋ : HyperEnv) : HyperEnv := 𝒢 ∪ ℋ
-
--- infixl:55 " |ₕ " => HyperEnv.merge
-
--- -- Merge identity
--- @[simp]
--- theorem HyperEnv.merge_unitL (𝒢 : HyperEnv) : ∅ |ₕ 𝒢 = 𝒢 := by
---   simp
-
--- @[simp]
--- theorem HyperEnv.merge_unitR (𝒢 : HyperEnv) : 𝒢 |ₕ ∅ = 𝒢 := by
---   simp
-
--- -- Merge commutative
--- @[simp]
--- theorem HyperEnv.merge_comm (𝒢 ℋ : HyperEnv) : 𝒢 |ₕ ℋ = ℋ |ₕ 𝒢 := by
---   simp [Finset.union_comm]
-
--- -- Merge associativity
--- @[simp]
--- theorem HyperEnv.merge_assoc (𝒢 ℋ 𝒦 : HyperEnv) :
---   (𝒢 |ₕ ℋ) |ₕ 𝒦 = 𝒢 |ₕ (ℋ |ₕ 𝒦) := by
---   simp
-
--- --------------------------------------- TYPING RULES ---------------------------------------
-
--- inductive Typing : HyperEnv → Proc → Prop where
---   | mix₀ :
---       ----------
---       Typing ∅ 𝟘
-
---   | mix {𝒢 ℋ : HyperEnv} {P Q : Proc} :
---       Typing 𝒢 P → Typing ℋ Q →
---       --------------------------
---       Typing (𝒢 |ₕ ℋ) (P |ₚ Q)
-
---   | cut (𝒢 : HyperEnv) (Γ Δ : Env) (P : Proc) (x y : PName) (A : Types) :
---       Typing (𝒢 |ₕ Γ‚ x ∶ A |ₕ Δ‚ y ∶ Aᗮ) P →
---       -----------------------------------------
---       Typing (𝒢 |ₕ Γ‚ Δ) (𝑣⸨x, y⸩ P)
-
---   | tensor {Γ Δ : Env} {P : Proc} {x y : PName} {B A : Types} :
---       Typing (Γ‚ y ∶ A |ₕ Δ‚ x ∶ B) P →
---       ------------------------------------
---       Typing (Γ‚ Δ‚ x ∶ A ⊗ B) (x⟦y⟧.P)
-
---   | one {P : Proc} {x : PName} :
---       Typing ∅ P →
---       ----------------------
---       Typing (x ∶ 1) (x⟦⟧.P)
-
---   | parr {Γ : Env} {P : Proc} {x y : PName} {A B : Types} :
---       Typing (Γ‚ y ∶ A‚ x ∶ B) P →
---       --------------------------------
---       Typing (Γ‚ x ∶ A ⅋ B) (x⸨y⸩.P)
-
---   | bot {Γ : Env} {P : Proc} {x : PName} :
---       Typing Γ P →
---       --------------------------
---       Typing (Γ‚ x ∶ ⊥) (x⸨⸩.P)
-
--- notation:50 "⊢ " P " ∷ " T => Typing T P
-
--- ----------------------------- TRANSITION RULES FOR DERIVATIONS -----------------------------
-
--- inductive Act : Type
---   | one     (x : PName)     -- x[]
---   | bot     (x : PName)     -- x()
---   | tensor  (x y : PName)   -- x[y]
---   | parr    (x y : PName)   -- x(y)
--- deriving Repr, DecidableEq
-
--- inductive Lbl : Type
---   | tau                       -- τ
---   | act   (a : Act)           -- l, for l ∈ Act
---   | par   (l l' : Act)        -- l | l' for l, l' ∈ Act
--- deriving Repr, DecidableEq
-
--- abbrev Lbls := List Lbl
-
--- instance : Coe Act Lbl := ⟨Lbl.act⟩
-
--- @[simp]
--- def getNamesOfLbl (func : Act → Finset PName) : Lbl → Finset PName
---   | .tau        => ∅                  -- names for τ
---   | .act a      => func a             -- names for l with l ∈ Act
---   | .par l l'   => func l ∪ func l'   -- names for l | l' with l, l' ∈ Act
-
--- @[simp]
--- def fNamesAct : Act -> Finset PName -- free names for a given action
---   | .one x | .bot x | .tensor x _ | .parr x _ => {x}
-
--- @[simp]
--- def Lbl.fNames : Lbl → Finset PName :=
---   getNamesOfLbl fNamesAct
-
--- @[simp]
--- def iNamesAct : Act → Finset PName -- introduced names for a given action
---   | .one _ | .bot _          => {}
---   | .tensor _ y | .parr _ y => {y}
-
--- @[simp]
--- def Lbl.iNames : Lbl → Finset PName :=
---   getNamesOfLbl iNamesAct
-
--- @[simp]
--- def Lbl.fresh (xs : List PName) (l : Lbl) :=
---   ∀ n ∈ xs, n ∉ l.fNames ∪ l.iNames
-
--- notation:80 x "⟦" y "⟧" => Act.tensor x y
--- notation:80 x "⟦⟧" => Act.one x
--- notation:80 x "⸨" y "⸩" => Act.parr x y
--- notation:80 x "⸨⸩" => Act.bot x
--- notation:70 "τ" => Lbl.tau
--- notation:70 l " |ₗ " l' => Lbl.par l l'
-
--- inductive TypingStep : {𝒢 : HyperEnv} → {P : Proc} → Typing 𝒢 P →
---   Lbl → {𝒢' : HyperEnv} → {P' : Proc} → Typing 𝒢' P' → Prop where
---   | one
---       {P : Proc} {x : PName} {𝒟 : Typing ∅ P} :
---       TypingStep (Typing.one 𝒟) (x⟦⟧) 𝒟
-
---   | tensor
---       {Γ Δ : Env} {P : Proc} {x x': PName} {A B : Types}
---       {𝒟 : Typing (Γ‚ x' ∶ A |ₕ Δ‚ x ∶ B) P} :
---       TypingStep (Typing.tensor 𝒟) (x⟦x'⟧) 𝒟
-
---   | bot
---       {Γ : Env} {P : Proc} {x : PName} {𝒟 : Typing {Γ} P} :
---       TypingStep (Typing.bot 𝒟) (x⸨⸩) 𝒟
-
---   | parr
---       {Γ : Env} {P : Proc} {x x' : PName} {A B : Types}
---       {𝒟 : Typing (Γ‚ x' ∶ A‚ x ∶ B) P} :
---       TypingStep (Typing.parr 𝒟) (x⸨x'⸩) 𝒟
-
---   | par₁
---       {𝒢 ℋ 𝒢': HyperEnv} {P Q P' : Proc} {l : Lbl}
---       {𝒟 : Typing 𝒢 P} {𝒟' : Typing 𝒢' P'} {ℰ : Typing ℋ Q}
---       (h : TypingStep 𝒟 l 𝒟') (disj : (l.iNames) ∩ (Q.fNames) = ∅) :
---       ---------------------------------------------------------------
---       TypingStep (Typing.mix 𝒟 ℰ) l (Typing.mix 𝒟' ℰ)
-
---   | par₂
---       {𝒢 ℋ ℋ': HyperEnv} {P Q Q' : Proc} {l : Lbl}
---       {𝒟 : Typing 𝒢 P} {ℰ : Typing ℋ Q} {ℰ' : Typing ℋ' Q'}
---       (h : TypingStep ℰ l ℰ') (disj : (l.iNames) ∩ (P.fNames) = ∅) :
---       ---------------------------------------------------------------
---       TypingStep (Typing.mix 𝒟 ℰ) l (Typing.mix 𝒟 ℰ')
-
---   | syn
---       {𝒢 𝒢' ℋ ℋ' : HyperEnv} {P P' Q Q' : Proc} {a a' : Act}
---       {𝒟 : Typing 𝒢 P} {𝒟' : Typing 𝒢' P'}
---       {ℰ : Typing ℋ Q} {ℰ' : Typing ℋ' Q'}
---       (h₁ : TypingStep 𝒟 a 𝒟')
---       (h₂ : TypingStep ℰ a' ℰ')
---       (disj : (a |ₗ a').iNames ∩ (P |ₚ Q).fNames = ∅) :
---       ---------------------------------------------------------------
---       TypingStep (Typing.mix 𝒟 ℰ) (a |ₗ a') (Typing.mix 𝒟' ℰ')
-
---   | alpha_equiv
---       {𝒢 𝒢' : HyperEnv} {P Q Q' : Proc} {l : Lbl}
---       {𝒟 : Typing 𝒢 P} {ℰ : Typing 𝒢 Q} {ℰ' : Typing 𝒢' Q'}
---       (h₁ : P =ₐ Q) (h₂ : TypingStep ℰ l ℰ') :
---       -------------------------------------------------------
---       TypingStep 𝒟 l ℰ'
-
---   | one_bot
---       {𝒢: HyperEnv} {Γ : Env} {P P' : Proc} {x y : PName}
---       {𝒟 : Typing (𝒢 |ₕ x ∶ 1 |ₕ Γ‚ y ∶ ⊥) P} {𝒟' : Typing (𝒢 |ₕ Γ) P'}
---       (h : TypingStep 𝒟 (x⟦⟧ |ₗ y⸨⸩) 𝒟') :
---       ----------------------------------------------------------------------
---       TypingStep (Typing.cut 𝒢 ∅ Γ P x y (1) 𝒟) (τ) 𝒟'
-
---   | tensor_parr
---       {𝒢 : HyperEnv} {Γ Δ Ξ : Env} {P P' : Proc} {x y x' y' : PName} {A B : Types}
---       {𝒟 : Typing (𝒢 |ₕ Γ‚ Δ‚ x ∶ A ⊗ B |ₕ Ξ‚ y ∶ Aᗮ ⅋ Bᗮ) P}
---       {𝒟' : Typing (𝒢 |ₕ Γ‚ x ∶ B |ₕ Δ‚ x' ∶ A |ₕ Ξ‚ y ∶ Bᗮ‚ y' ∶ Aᗮ) P'}
---       (h : TypingStep 𝒟 (x⟦x'⟧ |ₗ y⸨y'⸩) 𝒟') :
---       ----------------------------------------------------------------------------
---       TypingStep
---         (Typing.cut 𝒢 (Γ‚ Δ) Ξ P x y (A ⊗ B) 𝒟)
---         (τ)
---         (Typing.cut 𝒢 Γ (Δ‚ Ξ) (𝑣⸨x', y'⸩ P') x y B
---           (by
---            let inner := Typing.cut (𝒢 |ₕ {Γ‚ x ∶ B}) Δ (Ξ‚ y ∶ Bᗮ) P' x' y' A 𝒟'
---            rw [← Env.merge_assoc] at inner
---            exact inner
---           )
---         )
-
---   | res
---       {𝒢 𝒢': HyperEnv} {Γ Γ' Δ Δ' : Env} {P P' : Proc}
---       {x y : PName} {A : Types} {l : Lbl}
---       {𝒟 : Typing (𝒢 |ₕ Γ‚ x ∶ A |ₕ Δ‚ y ∶ Aᗮ) P}
---       {𝒟' : Typing (𝒢' |ₕ Γ'‚ x ∶ A |ₕ Δ'‚ y ∶ Aᗮ) P'}
---       (h : TypingStep 𝒟 l 𝒟')
---       (disj : l.fresh [x, y]) :
---       ----------------------------------------------------------------------------
---       TypingStep (Typing.cut 𝒢 Γ Δ P x y A 𝒟) l (Typing.cut 𝒢' Γ' Δ' P' x y A 𝒟')
-
--- notation:50 𝒟 " -[" l "]->ₜ " 𝒟' => TypingStep 𝒟 l 𝒟'
-
--- open Lean PrettyPrinter in
--- @[app_unexpander Lbl.act]
--- def unexpandLblAct : Unexpander
---   | `($_ $a) => pure a
---   | _ => pure Syntax.missing
-
--- -------------------------- MULTI-TYPING-STEP-TRANSITIONS ---------------------------
--- notation:80 "ε" => (List.nil : Lbls)
--- notation:60 xs " ∷ₗ " x => List.concat (xs : Lbls) (x : Lbl)
-
--- lemma eq_concat_nil {l} :
---   [l] = (ε ∷ₗ l) := by rfl
-
--- lemma cons_concat_eq {x xs y} :
---   x :: (xs ∷ₗ y) = x :: (xs ∷ₗ y) := by simp
-
--- lemma append_concat_eq {xs ys y} :
---   xs ++ (ys ∷ₗ y) = (xs ++ ys) ∷ₗ y := by simp
-
--- lemma cons_append_assoc {x : Lbl} {xs ys : Lbls} :
---   x :: (xs ++ ys) = (x :: xs) ++ ys := by rfl
-
--- inductive MTST : {𝒢 𝒢' : HyperEnv} → {P P' : Proc} →
---   Typing 𝒢 P → Lbls → Typing 𝒢' P' → Prop where
---   | refl
---     {𝒢 : HyperEnv} {P: Proc} {𝒟 : Typing 𝒢 P} :
---     MTST 𝒟 (ε) 𝒟
-
---   | stepR {l : Lbl} {ls : Lbls} {𝒢 𝒢' 𝒢'' : HyperEnv} {P P' P'' : Proc}
---     (𝒟  : Typing 𝒢  P) (𝒟' : Typing 𝒢' P') (𝒟'' : Typing 𝒢'' P'') :
---     (MTST 𝒟 ls 𝒟'') → (𝒟'' -[l]->ₜ 𝒟') →
---     -------------------------------------
---           MTST 𝒟 (ls ∷ₗ l) 𝒟'
-
--- notation:50 𝒟 " -[" ls "]->>ₜ " 𝒟' => MTST 𝒟 ls 𝒟'
-
--- ------------------------- PROC-FUCNTION & TRANSITION RULES -------------------------
-
--- def proc {𝒢 : HyperEnv} {P : Proc} (_ : ⊢ P ∷ 𝒢) : Proc := P
-
--- inductive ProcStep : (P : Proc) → Lbl → (P' : Proc) → Prop where
---   | one
---       {P : Proc} {x : PName} :
---       ProcStep (x⟦⟧.P) (x⟦⟧) P
-
---   | tensor
---       {P : Proc} {x x' : PName} :
---       ProcStep (x⟦x'⟧.P) (x⟦x'⟧) P
-
---   | bot
---       {P : Proc} {x : PName} :
---       ProcStep (x⸨⸩.P) (x⸨⸩) P
-
---   | parr
---       {P : Proc} {x x' : PName} :
---       ProcStep (x⸨x'⸩.P) (x⸨x'⸩) P
-
---   | par₁
---       {P P' Q : Proc} {l : Lbl} :
---       ProcStep P l P' → l.iNames ∩ Q.fNames = ∅ →
---       -------------------------------------------
---       ProcStep (P |ₚ Q) l (P' |ₚ Q)
-
---   | par₂
---       {P Q Q' : Proc} {l : Lbl} :
---       ProcStep Q l Q' → l.iNames ∩ P.fNames = ∅ →
---       --------------------------------------------
---       ProcStep (P |ₚ Q) l (P |ₚ Q')
-
---   | syn
---       {P P' Q Q' : Proc} {l l' : Act} :
---       ProcStep P l P' → ProcStep Q l' Q' →
---       (l |ₗ l').iNames ∩ (P |ₚ Q).fNames = ∅  →
---       ----------------------------------------
---       ProcStep (P |ₚ Q) (l |ₗ l') (P' |ₚ Q')
-
---   | alpha_equiv
---       {P Q Q' : Proc} {l : Lbl} :
---       (P =ₐ Q) → ProcStep Q l Q' →
---       -------------------------------
---       ProcStep P l Q'
-
---   | one_bot
---       {P P' : Proc} {x y : PName} :
---       ProcStep P (x⟦⟧ |ₗ y⸨⸩) P' →
---       --------------------------------------
---       ProcStep (𝑣⸨x, y⸩ P) (τ) P'
-
---   | tensor_parr
---       {P P' : Proc} {x x' y y' : PName} :
---       ProcStep P (x⟦x'⟧ |ₗ y⸨y'⸩) P' →
---       --------------------------------------------------------------------
---       ProcStep (𝑣⸨x, y⸩ P) (τ) (𝑣⸨x, y⸩ (𝑣⸨x', y'⸩ P'))
-
---   | res
---       {P P' : Proc} {x y : PName} {l : Lbl} :
---       ProcStep P l P' → l.fresh [x, y] →
---       -------------------------------------
---       ProcStep (𝑣⸨x, y⸩ P) (l) (𝑣⸨x, y⸩ P')
-
--- notation:50 P " -[" l "]->ₚ " P' => ProcStep P l P'
-
--- inductive MPST : (P : Proc) → Lbls → (P' : Proc) → Prop where
---   | refl
---     {P : Proc} :
---     ------------
---     MPST P (ε) P
-
---   | stepR {l : Lbl} {ls : Lbls} {P P'' P' : Proc} :
---     (MPST P ls P'') → (P'' -[l]->ₚ P') →
---     ----------------------------------
---           MPST P (ls ∷ₗ l) P'
-
--- notation:50 P " -[" ls "]->>ₚ " P' => MPST P ls P'
-
--- ------------------------- ENV-FUCNTION & TRANSITION RULES --------------------------
-
--- def env {𝒢 : HyperEnv} {P : Proc} (_ : ⊢ P ∷ 𝒢) : HyperEnv := 𝒢
-
--- inductive EnvStep : HyperEnv → Lbl → HyperEnv → Prop where
---   | one
---       {x : PName} :
---       EnvStep (x ∶ 1) (x⟦⟧) ∅
-
---   | tensor
---       {Γ Δ : Env} {x x' : PName} {A B : Types} :
---       EnvStep (Γ‚ Δ‚ x ∶ A ⊗ B) (x⟦x'⟧) (Γ‚ x'∶ A |ₕ Δ‚ x ∶ B)
-
---   | bot
---       {Γ : Env} {x : PName} :
---       EnvStep (Γ‚ x ∶ ⊥) (x⸨⸩) Γ
-
---   | parr
---       {Γ Δ : Env} {x x' : PName} {A B : Types} :
---       EnvStep (Γ‚ x ∶ A ⅋ B) (x⸨x'⸩) (Γ‚ x' ∶ A‚ Δ‚ x ∶ B)
-
---   | par₁
---       {𝒢 𝒢' ℋ : HyperEnv} {l : Lbl} :
---       EnvStep 𝒢 l 𝒢' →
---       -----------------------------
---       EnvStep (𝒢 |ₕ ℋ) l (𝒢' |ₕ ℋ)
-
---   | par₂
---       {𝒢 ℋ ℋ': HyperEnv} {l : Lbl} :
---       EnvStep ℋ l ℋ' →
---       -----------------------------
---       EnvStep (𝒢 |ₕ ℋ) l (𝒢 |ₕ ℋ')
-
---   | syn
---       {𝒢 𝒢' ℋ ℋ': HyperEnv} {l l' : Act} :
---       EnvStep 𝒢 l 𝒢' → EnvStep ℋ l' ℋ' →
---       ------------------------------------
---       EnvStep (𝒢 |ₕ ℋ) (l |ₗ l') (𝒢' |ₕ ℋ')
-
---   | one_bot
---       {𝒢 : HyperEnv} {Γ : Env} {x y : PName} :
---       EnvStep (𝒢 |ₕ x ∶ 1 |ₕ Γ‚ y ∶ ⊥) (x⟦⟧ |ₗ y⸨⸩) (𝒢 |ₕ Γ) →
---       ----------------------------------------------------------
---       EnvStep (𝒢 |ₕ Γ) (τ) (𝒢 |ₕ Γ)
-
---   | tensor_parr
---       {𝒢 : HyperEnv} {Γ Δ Ξ : Env} {x x' y y': PName} {A B : Types} :
---       EnvStep
---         (𝒢 |ₕ Γ‚ Δ‚ x ∶ A ⊗ B |ₕ Ξ‚ y ∶ Aᗮ ⅋ Bᗮ)
---         (x⟦x'⟧ |ₗ y⸨y'⸩)
---         (𝒢 |ₕ Γ‚ x' ∶ A |ₕ Δ‚ x ∶ B |ₕ Ξ‚ y' ∶ Aᗮ‚ y ∶ Bᗮ) →
---       --------------------------------------------------------
---       EnvStep (𝒢 |ₕ Γ‚ Δ‚ Ξ) (τ) (𝒢 |ₕ Γ‚ Δ‚ Ξ)
-
---   | res
---       {𝒢 𝒢' : HyperEnv} {Γ Γ' Δ Δ' : Env} {x y : PName} {A B : Types} {l : Lbl} :
---       EnvStep (𝒢 |ₕ Γ‚ x ∶ Aᗮ |ₕ Δ‚ y ∶ A) (l) (𝒢' |ₕ Γ'‚ x ∶ Aᗮ |ₕ Δ'‚ y ∶ A) →
---       ----------------------------------------------------------------------------
---       EnvStep (𝒢 |ₕ Γ‚ Δ) l (𝒢' |ₕ Γ'‚ Δ')
-
--- notation:50 P " -[" l "]->ₑ " P' => EnvStep P l P'
-
--- inductive MEST : (𝒢 : HyperEnv) → Lbls → (𝒢' : HyperEnv) → Prop where
---   | refl
---     {𝒢 : HyperEnv} :
---     ------------
---     MEST 𝒢 (ε) 𝒢
-
---   | stepR {l : Lbl} {ls : Lbls} {𝒢 𝒢'' 𝒢' : HyperEnv} :
---     (MEST 𝒢 ls 𝒢'') → (𝒢'' -[l]->ₑ 𝒢') →
---     ----------------------------------
---           MEST 𝒢 (ls ∷ₗ l) 𝒢'
-
--- notation:50 𝒢 " -[" ls "]->>ₑ " 𝒢' => MPST 𝒢 ls 𝒢'
+-- Merge identity
+@[simp]
+theorem Env.merge_unitR (Δ : Env) : Δ‚ ∅ = Δ := by
+  simp
+
+@[simp]
+theorem Env.merge_unitL (Δ : Env) : ∅‚ Δ = Δ := by
+  simp
+
+-- Merge commutivity
+-- theorem mergeEnv.comm (Δ Γ : Env) : disjointEnv Δ Γ → mergeEnv Δ Γ = mergeEnv Γ Δ := by
+@[simp]
+theorem Env.merge_comm (Δ Γ : Env) : Δ‚ Γ = Γ‚ Δ := by
+  simp [Finset.union_comm]
+
+-- Merge associativity
+@[simp]
+theorem Env.merge_assoc (Δ Γ Ε : Env) : Δ‚ Γ‚ Ε = Δ‚ (Γ‚ Ε) := by
+  simp
+
+@[simp]
+lemma Env.merge_swap_last (Γ Δ Ξ : Env) :
+  (Γ‚ Δ)‚ Ξ = (Γ‚ Ξ)‚ Δ := by
+  rw [Env.merge_comm, ←Env.merge_assoc]
+  conv => lhs ; lhs ; rw [Env.merge_comm]
+
+@[simp]
+lemma Env.merge_move_last_two_left (Γ Δ Ξ Ε : Env) :
+  Γ‚ Δ‚ Ξ‚ Ε = Γ‚ Ε‚ Δ‚ Ξ := by
+  rw [Env.merge_swap_last, Env.merge_swap_last Γ Δ Ε]
+
+@[simp]
+lemma Env.merge_move_second_two_right (Γ Δ Ξ Ε : Env) :
+  Γ‚ Δ‚ Ξ‚ Ε = Γ‚ Ξ‚ Ε‚ Δ := by
+  rw [Env.merge_swap_last Γ Δ Ξ, Env.merge_swap_last]
+
+
+------------------------------------ HYPER-ENVIRONMENTS ------------------------------------
+
+abbrev HyperEnv := Finset (Env)
+
+abbrev EmptyHyperEnv : HyperEnv := ∅
+
+instance : Coe Env HyperEnv := ⟨fun Γ => ({Γ} : HyperEnv)⟩
+
+/- FIXME: eval does not work since non-computable -/
+open Lean in
+noncomputable instance : Repr HyperEnv where
+  reprPrec (𝒢 : HyperEnv) _ :=
+    if 𝒢 = ∅ then "∅"
+    else
+      let entries := 𝒢.toList.map repr
+      Format.joinSep entries " |ₕ "
+
+noncomputable instance : ToString HyperEnv where
+  toString g := reprStr g
+
+def pairwise {α : Type} (r : α → α → Prop) (s : Finset α) : Prop :=
+  ∀ x ∈ s, ∀ y ∈ s, y ≠ x → r x y
+
+def HyperEnv.linear (𝒢 : HyperEnv) : Prop :=
+  ∀ Δ ∈ 𝒢, Δ.linear ∧                               -- ensure each env is linear
+  pairwise (fun Δ Γ => Δ.disjoint Γ) 𝒢              -- ensure pairwise env disjointness
+
+def HyperEnv.names (𝒢 : HyperEnv) : Finset PName :=
+  Finset.fold (· ∪ ·) ∅ Env.names 𝒢
+
+-- Lookup method for finding the type of a name in the hyperenvironment
+noncomputable def HyperEnv.lookup (𝒢 : HyperEnv) (x : PName) : Option Types :=
+  (𝒢.toList.find? (fun Δ => Δ⸨x⸩ₑ ≠ none)) >>= fun Δ  => Δ⸨x⸩ₑ
+
+notation:60 𝒢 "⸨" x "⸩ₕ" => HyperEnv.lookup 𝒢 x
+
+def HyperEnv.disjoint (𝒢 ℋ : HyperEnv) : Prop :=
+  -- 1. ensure both hyperenvs are lienar
+  -- 2. ensure disjoint env names
+  -- 3. ensure no duplicate definitions across hyperenvs
+    -- s.t. an unambigous lookup in the individual hyperenvs
+    -- yields an unambigous lookupin the merged hyperenv
+    -- i.e. the intersection of their defined names is empty
+  𝒢.linear ∧ ℋ.linear ∧
+  (𝒢 ∩ ℋ).card = 0 ∧
+  (𝒢.names ∩ ℋ.names).card = 0
+
+-- Order independent equality for hyper-environments
+@[simp]
+def HyperEnv.Eq (𝒢 ℋ : HyperEnv) : Prop :=
+  -- (1) 𝒢 and ℋ must define the same names
+  -- (2) The typing of all defined names must match i.e. ∀ x, 𝒢(x) = ℋ(x)
+  HyperEnv.names 𝒢 = HyperEnv.names ℋ ∧
+  ∀ x ∈ HyperEnv.names 𝒢, 𝒢⸨x⸩ₕ = ℋ⸨x⸩ₕ
+
+notation 𝒢 " =ₕ " ℋ => HyperEnv.Eq 𝒢 ℋ
+
+-- Eq reflexivity
+@[simp]
+theorem HyperEnv.Eq_refl (𝒢 : HyperEnv) : 𝒢 =ₕ 𝒢 := by
+  simp
+
+-- Eq symmetry
+@[simp]
+theorem HyperEnv.Eq_symm (𝒢 ℋ : HyperEnv) (h : 𝒢 =ₕ ℋ) : ℋ =ₕ 𝒢 := by
+  rcases h with ⟨h_names, h_vals⟩
+  refine ⟨h_names.symm, ?vals⟩
+  intro x hx
+  rw [h_names] at h_vals
+  apply (h_vals x hx).symm
+
+-- Eq transitivity
+@[simp]
+theorem HyperEnv.Eq_trans (𝒢 ℋ 𝒦 : HyperEnv) (h₁ : 𝒢 =ₕ ℋ) (h₂ : ℋ =ₕ 𝒦) :
+  𝒢 =ₕ 𝒦 := by
+  rcases h₁ with ⟨h₁_names, h₁_vals⟩
+  rcases h₂ with ⟨h₂_names, h₂_vals⟩
+  refine ⟨?names, ?vals⟩
+  · rw [h₁_names, h₂_names]
+  · intro x hx
+    have hxH : x ∈ ℋ.names := by rw [← h₁_names]; exact hx
+    calc
+      𝒢⸨x⸩ₕ = ℋ⸨x⸩ₕ := h₁_vals x hx
+      _          = 𝒦⸨x⸩ₕ := h₂_vals x hxH
+
+instance : Equivalence HyperEnv.Eq :=
+⟨HyperEnv.Eq_refl, @HyperEnv.Eq_symm, @HyperEnv.Eq_trans⟩
+
+@[simp]
+abbrev HyperEnv.merge (𝒢 ℋ : HyperEnv) : HyperEnv := 𝒢 ∪ ℋ
+
+infixl:55 " |ₕ " => HyperEnv.merge
+
+-- Merge identity
+@[simp]
+theorem HyperEnv.merge_unitL (𝒢 : HyperEnv) : ∅ |ₕ 𝒢 = 𝒢 := by
+  simp
+
+@[simp]
+theorem HyperEnv.merge_unitR (𝒢 : HyperEnv) : 𝒢 |ₕ ∅ = 𝒢 := by
+  simp
+
+-- Merge commutative
+@[simp]
+theorem HyperEnv.merge_comm (𝒢 ℋ : HyperEnv) : 𝒢 |ₕ ℋ = ℋ |ₕ 𝒢 := by
+  simp [Finset.union_comm]
+
+-- Merge associativity
+@[simp]
+theorem HyperEnv.merge_assoc (𝒢 ℋ 𝒦 : HyperEnv) :
+  (𝒢 |ₕ ℋ) |ₕ 𝒦 = 𝒢 |ₕ (ℋ |ₕ 𝒦) := by
+  simp
+
+--------------------------------------- TYPING RULES ---------------------------------------
+
+inductive Typing : HyperEnv → Proc → Prop where
+  | mix₀ :
+      ----------
+      Typing ∅ 𝟘
+
+  | mix {𝒢 ℋ : HyperEnv} {P Q : Proc} :
+      Typing 𝒢 P → Typing ℋ Q →
+      --------------------------
+      Typing (𝒢 |ₕ ℋ) (P |ₚ Q)
+
+  | cut (𝒢 : HyperEnv) (Γ Δ : Env) (P : Proc) (x y : PName) (A : Types) :
+      Typing (𝒢 |ₕ Γ‚ x ∶ A |ₕ Δ‚ y ∶ Aᗮ) P →
+      -----------------------------------------
+      Typing (𝒢 |ₕ Γ‚ Δ) (𝑣⸨x, y⸩ P)
+
+  | tensor {Γ Δ : Env} {P : Proc} {x y : PName} {B A : Types} :
+      Typing (Γ‚ y ∶ A |ₕ Δ‚ x ∶ B) P →
+      ------------------------------------
+      Typing (Γ‚ Δ‚ x ∶ A ⊗ B) (x⟦y⟧.P)
+
+  | one {P : Proc} {x : PName} :
+      Typing ∅ P →
+      ----------------------
+      Typing (x ∶ 1) (x⟦⟧.P)
+
+  | parr {Γ : Env} {P : Proc} {x y : PName} {A B : Types} :
+      Typing (Γ‚ y ∶ A‚ x ∶ B) P →
+      --------------------------------
+      Typing (Γ‚ x ∶ A ⅋ B) (x⸨y⸩.P)
+
+  | bot {Γ : Env} {P : Proc} {x : PName} :
+      Typing Γ P →
+      --------------------------
+      Typing (Γ‚ x ∶ ⊥) (x⸨⸩.P)
+
+notation:50 "⊢ " P " ∷ " T => Typing T P
+
+----------------------------- TRANSITION RULES FOR DERIVATIONS -----------------------------
+
+inductive Mu : Type
+  | L | R | DISP | DUP | USE
+deriving Repr, DecidableEq
+
+inductive Act : Type
+  | one       (x : PName)               -- x[]
+  | bot       (x : PName)               -- x()
+  | tensor    (x y : PName)             -- x[y]
+  | parr      (x y : PName)             -- x(y)
+  | output    (x : PName) (A : Types)   -- x[A]
+  | input     (x : PName) (A : Types)   -- x(X)
+  | muBrack   (x : PName) (μ : Mu)      -- x[μ]
+  | muParen   (x : PName) (μ : Mu)      -- x[μ]
+deriving Repr, DecidableEq
+
+@[simp]
+def fNamesAct : Act -> Finset PName -- free names
+  | .one x | .bot x
+  | .tensor x _ | .parr x _
+  | .input x _ | .output x _
+  | .muBrack x _  | .muParen x _ => {x}
+
+@[simp]
+def iNamesAct : Act → Finset PName -- introduced names
+  | .one _ | .bot _ | .input _ _ | .output _ _
+  | Act.muBrack _ _ | Act.muParen _ _ => {}
+  | .tensor _ y | .parr _ y => {y}
+
+inductive Lbl : Type
+  | tau                   -- τ
+  | link  (x y : PName)   -- x ⟷ y
+  | act   (p : Act)       -- l, for l ∈ Act
+  | par   (l l' : Act)    -- l | l' for l, l' ∈ Act, missing: i(l) ∩ i(l') = ∅
+deriving Repr, DecidableEq
+
+abbrev Lbls := List Lbl
+
+instance : Coe Act Lbl := ⟨Lbl.act⟩
+
+def Lbl.WF : Lbl → Prop
+  | .tau => true
+  | .link _ _ => true
+  | .act _ => true
+  | .par l l' => (iNamesAct l) ∩ (iNamesAct l') = ∅
+
+@[simp]
+def Lbl.fNames : Lbl → Finset PName
+  | .tau        => ∅
+  | .link x y   => {x, y}
+  | .act a      => fNamesAct a
+  | .par l l'   => fNamesAct l ∪ fNamesAct l'
+
+@[simp]
+def Lbl.iNames : Lbl → Finset PName
+  | .tau        => ∅
+  | .link _ _   => {}
+  | .act a      => iNamesAct a
+  | .par l l'   => iNamesAct l ∪ iNamesAct l'
+
+@[simp]
+def Lbl.fresh (xs : List PName) (l : Lbl) :=
+  ∀ n ∈ xs, n ∉ l.fNames ∪ l.iNames
+
+notation:80 x "⟦" y "⟧" => Act.tensor x y
+notation:80 x "⟦⟧" => Act.one x
+notation:80 x "⸨" y "⸩" => Act.parr x y
+notation:80 x "⸨⸩" => Act.bot x
+notation:80 "τ" => Lbl.tau
+notation:80 x "⟷ₗ" y => Lbl.link x y
+notation:70 l " |ₗ " l' => Lbl.par l l'
+notation:80 x "⟦" A "⟧:" => Act.output x A
+notation:80 x "⸨" X "⸩:" => Act.input x X
+
+notation:80 x "⟦𝐋⟧" => Act.muBrack x Mu.L
+notation:80 x "⸨𝐋⸩" => Act.muParen x Mu.L
+notation:80 x "⟦𝐑⟧" => Act.muBrack x Mu.R
+notation:80 x "⸨𝐑⸩" => Act.muParen x Mu.R
+notation:80 x "⟦USE⟧" => Act.muBrack x Mu.USE
+notation:80 x "⸨USE⸩" => Act.muParen x Mu.USE
+notation:80 x "⟦DUP⟧" => Act.muBrack x Mu.DUP
+notation:80 x "⸨DUP⸩" => Act.muParen x Mu.DUP
+notation:80 x "⟦DISP⟧" => Act.muBrack x Mu.DISP
+notation:80 x "⸨DISP⸩" => Act.muParen x Mu.DISP
+
+notation:80 x "⟦" μ "⟧ₘ" => Act.muBrack x μ
+notation:80 x "⸨" μ "⸩ₘ" => Act.muParen x μ
+
+inductive TypingStep : {𝒢 : HyperEnv} → {P : Proc} → Typing 𝒢 P →
+  Lbl → {𝒢' : HyperEnv} → {P' : Proc} → Typing 𝒢' P' → Prop where
+  | one
+      {P : Proc} {x : PName} {𝒟 : Typing ∅ P} :
+      TypingStep (Typing.one 𝒟) (x⟦⟧) 𝒟
+
+  | tensor
+      {Γ Δ : Env} {P : Proc} {x x': PName} {A B : Types}
+      {𝒟 : Typing (Γ‚ x' ∶ A |ₕ Δ‚ x ∶ B) P} :
+      TypingStep (Typing.tensor 𝒟) (x⟦x'⟧) 𝒟
+
+  | bot
+      {Γ : Env} {P : Proc} {x : PName} {𝒟 : Typing {Γ} P} :
+      TypingStep (Typing.bot 𝒟) (x⸨⸩) 𝒟
+
+  | parr
+      {Γ : Env} {P : Proc} {x x' : PName} {A B : Types}
+      {𝒟 : Typing (Γ‚ x' ∶ A‚ x ∶ B) P} :
+      TypingStep (Typing.parr 𝒟) (x⸨x'⸩) 𝒟
+
+  | par₁
+      {𝒢 ℋ 𝒢': HyperEnv} {P Q P' : Proc} {l : Lbl}
+      {𝒟 : Typing 𝒢 P} {𝒟' : Typing 𝒢' P'} {ℰ : Typing ℋ Q}
+      (h : TypingStep 𝒟 l 𝒟') (disj : (l.iNames) ∩ (Q.fNames) = ∅) :
+      ---------------------------------------------------------------
+      TypingStep (Typing.mix 𝒟 ℰ) l (Typing.mix 𝒟' ℰ)
+
+  | par₂
+      {𝒢 ℋ ℋ': HyperEnv} {P Q Q' : Proc} {l : Lbl}
+      {𝒟 : Typing 𝒢 P} {ℰ : Typing ℋ Q} {ℰ' : Typing ℋ' Q'}
+      (h : TypingStep ℰ l ℰ') (disj : (l.iNames) ∩ (P.fNames) = ∅) :
+      ---------------------------------------------------------------
+      TypingStep (Typing.mix 𝒟 ℰ) l (Typing.mix 𝒟 ℰ')
+
+  | syn
+      {𝒢 𝒢' ℋ ℋ' : HyperEnv} {P P' Q Q' : Proc} {l l' : Act}
+      {𝒟 : Typing 𝒢 P} {𝒟' : Typing 𝒢' P'}
+      {ℰ : Typing ℋ Q} {ℰ' : Typing ℋ' Q'}
+      (h₁ : TypingStep 𝒟 l 𝒟')
+      (h₂ : TypingStep ℰ l' ℰ')
+      (disj : (l |ₗ l').iNames ∩ (P |ₚ Q).fNames = ∅)
+      (WF : (l |ₗ l').WF) : -- Don't know how to show TypingStep preserves WF without this
+      ---------------------------------------------------------
+      TypingStep (Typing.mix 𝒟 ℰ) (l |ₗ l') (Typing.mix 𝒟' ℰ')
+
+  | alpha_equiv
+      {𝒢 𝒢' : HyperEnv} {P Q Q' : Proc} {l : Lbl}
+      {𝒟 : Typing 𝒢 P} {ℰ : Typing 𝒢 Q} {ℰ' : Typing 𝒢' Q'}
+      (h₁ : P =ₐ Q) (h₂ : TypingStep ℰ l ℰ') :
+      -------------------------------------------------------
+      TypingStep 𝒟 l ℰ'
+
+  | one_bot
+      {𝒢: HyperEnv} {Γ : Env} {P P' : Proc} {x y : PName}
+      {𝒟 : Typing (𝒢 |ₕ x ∶ 1 |ₕ Γ‚ y ∶ ⊥) P} {𝒟' : Typing (𝒢 |ₕ Γ) P'}
+      (h : TypingStep 𝒟 (x⟦⟧ |ₗ y⸨⸩) 𝒟') :
+      ----------------------------------------------------------------
+      TypingStep (Typing.cut 𝒢 ∅ Γ P x y (1) 𝒟) (τ) 𝒟'
+
+  | tensor_parr
+      {𝒢 : HyperEnv} {Γ Δ Ξ : Env} {P P' : Proc} {x y x' y' : PName} {A B : Types}
+      {𝒟 : Typing (𝒢 |ₕ Γ‚ Δ‚ x ∶ A ⊗ B |ₕ Ξ‚ y ∶ Aᗮ ⅋ Bᗮ) P}
+      {𝒟' : Typing (𝒢 |ₕ Γ‚ x ∶ B |ₕ Δ‚ x' ∶ A |ₕ Ξ‚ y ∶ Bᗮ‚ y' ∶ Aᗮ) P'}
+      (h : TypingStep 𝒟 (x⟦x'⟧ |ₗ y⸨y'⸩) 𝒟') :
+      ----------------------------------------------------------------------------
+      TypingStep
+        (Typing.cut 𝒢 (Γ‚ Δ) Ξ P x y (A ⊗ B) 𝒟)
+        (τ)
+        (Typing.cut 𝒢 Γ (Δ‚ Ξ) (𝑣⸨x', y'⸩ P') x y B
+          (by
+           let inner := Typing.cut (𝒢 |ₕ {Γ‚ x ∶ B}) Δ (Ξ‚ y ∶ Bᗮ) P' x' y' A 𝒟'
+           rw [← Env.merge_assoc] at inner
+           exact inner
+          )
+        )
+
+  | res
+      {𝒢 𝒢': HyperEnv} {Γ Γ' Δ Δ' : Env} {P P' : Proc}
+      {x y : PName} {A : Types} {l : Lbl}
+      {𝒟 : Typing (𝒢 |ₕ Γ‚ x ∶ A |ₕ Δ‚ y ∶ Aᗮ) P}
+      {𝒟' : Typing (𝒢' |ₕ Γ'‚ x ∶ A |ₕ Δ'‚ y ∶ Aᗮ) P'}
+      (h : TypingStep 𝒟 l 𝒟') (disj : l.fresh [x, y]) :
+      ----------------------------------------------------------------------------
+      TypingStep (Typing.cut 𝒢 Γ Δ P x y A 𝒟) l (Typing.cut 𝒢' Γ' Δ' P' x y A 𝒟')
+
+notation:50 𝒟 " -[" l "]->ₜ " 𝒟' => TypingStep 𝒟 l 𝒟'
+
+open Lean PrettyPrinter in
+@[app_unexpander Lbl.act]
+def unexpandLblAct : Unexpander
+  | `($_ $a) => pure a
+  | _ => pure Syntax.missing
+
+theorem TypingStep.preserves_WF (Γ Γ' : HyperEnv) (P P' : Proc)
+  (𝒟 : ⊢ P ∷ Γ) (𝒟' : ⊢ P' ∷ Γ') (l : Lbl) :
+  TypingStep 𝒟 l 𝒟' → l.WF := by
+  intro h
+  induction h
+  case one | bot | tensor | parr | one_bot | tensor_parr => simp [Lbl.WF]
+  case par₁ | par₂| alpha_equiv | res => simp_all
+  case syn WF ih1 ih2 => exact WF
+
+-------------------------- MULTI-TYPING-STEP-TRANSITIONS ---------------------------
+notation:80 "ε" => (List.nil : Lbls)
+notation:60 xs " ∷ₗ " x => List.concat (xs : Lbls) (x : Lbl)
+
+lemma eq_concat_nil {l} :
+  [l] = (ε ∷ₗ l) := by rfl
+
+lemma cons_concat_eq {x xs y} :
+  x :: (xs ∷ₗ y) = x :: (xs ∷ₗ y) := by simp
+
+lemma append_concat_eq {xs ys y} :
+  xs ++ (ys ∷ₗ y) = (xs ++ ys) ∷ₗ y := by simp
+
+lemma cons_append_assoc {x : Lbl} {xs ys : Lbls} :
+  x :: (xs ++ ys) = (x :: xs) ++ ys := by rfl
+
+inductive MTST : {𝒢 𝒢' : HyperEnv} → {P P' : Proc} →
+  Typing 𝒢 P → Lbls → Typing 𝒢' P' → Prop where
+  | refl
+    {𝒢 : HyperEnv} {P: Proc} {𝒟 : Typing 𝒢 P} :
+    MTST 𝒟 (ε) 𝒟
+
+  | stepR {l : Lbl} {ls : Lbls} {𝒢 𝒢' 𝒢'' : HyperEnv} {P P' P'' : Proc}
+    (𝒟  : Typing 𝒢  P) (𝒟' : Typing 𝒢' P') (𝒟'' : Typing 𝒢'' P'') :
+    (MTST 𝒟 ls 𝒟'') → (𝒟'' -[l]->ₜ 𝒟') →
+    -------------------------------------
+          MTST 𝒟 (ls ∷ₗ l) 𝒟'
+
+notation:50 𝒟 " -[" ls "]->>ₜ " 𝒟' => MTST 𝒟 ls 𝒟'
+
+------------------------- PROC-FUCNTION & TRANSITION RULES -------------------------
+
+def proc {𝒢 : HyperEnv} {P : Proc} (_ : ⊢ P ∷ 𝒢) : Proc := P
+
+inductive ProcStep : (P : Proc) → Lbl → (P' : Proc) → Prop where
+  | one
+      {P : Proc} {x : PName} :
+      ProcStep (x⟦⟧.P) (x⟦⟧) P
+
+  | tensor
+      {P : Proc} {x x' : PName} :
+      ProcStep (x⟦x'⟧.P) (x⟦x'⟧) P
+
+  | bot
+      {P : Proc} {x : PName} :
+      ProcStep (x⸨⸩.P) (x⸨⸩) P
+
+  | parr
+      {P : Proc} {x x' : PName} :
+      ProcStep (x⸨x'⸩.P) (x⸨x'⸩) P
+
+  | par₁
+      {P P' Q : Proc} {l : Lbl} :
+      ProcStep P l P' → l.iNames ∩ Q.fNames = ∅ →
+      -------------------------------------------
+      ProcStep (P |ₚ Q) l (P' |ₚ Q)
+
+  | par₂
+      {P Q Q' : Proc} {l : Lbl} :
+      ProcStep Q l Q' → l.iNames ∩ P.fNames = ∅ →
+      --------------------------------------------
+      ProcStep (P |ₚ Q) l (P |ₚ Q')
+
+  | syn
+      {P P' Q Q' : Proc} {l l' : Act} :
+      ProcStep P l P' → ProcStep Q l' Q' →
+      (l |ₗ l').iNames ∩ (P |ₚ Q).fNames = ∅  →
+      ----------------------------------------
+      ProcStep (P |ₚ Q) (l |ₗ l') (P' |ₚ Q')
+
+  | alpha_equiv
+      {P Q Q' : Proc} {l : Lbl} :
+      (P =ₐ Q) → ProcStep Q l Q' →
+      -------------------------------
+      ProcStep P l Q'
+
+  | one_bot
+      {P P' : Proc} {x y : PName} :
+      ProcStep P (x⟦⟧ |ₗ y⸨⸩) P' →
+      ----------------------------
+      ProcStep (𝑣⸨x, y⸩ P) (τ) P'
+
+  | tensor_parr
+      {P P' : Proc} {x x' y y' : PName} :
+      ProcStep P (x⟦x'⟧ |ₗ y⸨y'⸩) P' →
+      -------------------------------------------------
+      ProcStep (𝑣⸨x, y⸩ P) (τ) (𝑣⸨x, y⸩ (𝑣⸨x', y'⸩ P'))
+
+  | res
+      {P P' : Proc} {x y : PName} {l : Lbl} :
+      ProcStep P l P' → l.fresh [x, y] →
+      -------------------------------------
+      ProcStep (𝑣⸨x, y⸩ P) (l) (𝑣⸨x, y⸩ P')
+
+  | output
+      {P : Proc} {x : PName} {X : Types} :
+      ProcStep (x⟦X⟧:P) (x⟦X⟧:) P
+
+  -- | dispParen
+
+  | disposeBrack
+      {P : Proc} {x : PName} :
+      ProcStep (x⟦DISP⟧.P) (x⟦DISP⟧) (x⸨⸩.P)
+
+  -- | dupParen
+
+  | dupBrack
+      {P : Proc} {x x' : PName} :
+      ProcStep (x⟦DUP⟧⸨x'⸩.P) (x⟦DUP⟧) (x⸨x'⸩.P)
+
+  | useParen
+      {P : Proc} {x : PName} :
+      ProcStep (!x.⦃P⦄) (x⸨USE⸩) P
+
+  | useBrack
+      {P : Proc} {x : PName} :
+      ProcStep (x⟦USE⟧.P) (x⟦USE⟧) P
+
+  | input -- FIXME: missing the replace A with X thingy
+      {P : Proc} {x : PName} {A X : Types}:
+      ProcStep (x⸨X⸩:P) (x⸨A⸩:) P --{A/X}
+
+  | selectL
+      {P : Proc} {x : PName} :
+      ProcStep (x⟦𝐋⟧.P) (x⟦𝐋⟧) P
+
+  | recieveL
+      {P Q : Proc} {x : PName} :
+      ProcStep (⸨x⸩.case⦃𝐋 : P, 𝐑 : Q⦄) (x⸨𝐋⸩) P
+
+  | selectR
+      {P : Proc} {x : PName} :
+      ProcStep (x⟦𝐑⟧.P) (x⟦𝐑⟧) P
+
+  | recieveR
+      {P Q : Proc} {x : PName} :
+      ProcStep (⸨x⸩.case⦃𝐋 : P, 𝐑 : Q⦄) (x⸨𝐑⸩) Q
+
+  | link₁
+      {x y : PName} :
+      ProcStep (x ⟷ₚ y) (x ⟷ₗ y) 𝟘
+
+  | link₂
+      {x y : PName} :
+      ProcStep (x ⟷ₚ y) (y ⟷ₗ x) 𝟘
+
+  | com {P P' : Proc} {x y : PName} {μ : Mu} :
+      ProcStep P (x⟦μ⟧ₘ |ₗ y⟦μ⟧ₘ) P' →
+      ----------------------------------------
+      ProcStep (𝑣⸨x, y⸩ P) (τ) (𝑣⸨x, y⸩ P')
+
+  | axcut -- FIXME: missing the replacement syntax thingy
+      {P P' : Proc} {x y z : PName} :
+      ProcStep P (x ⟷ₗ y) P' →
+      -------------------------------------
+      ProcStep (𝑣⸨y, z⸩ P) (τ) P' -- {x/z}
+
+notation:50 P " -[" l "]->ₚ " P' => ProcStep P l P'
+
+inductive MPST : (P : Proc) → Lbls → (P' : Proc) → Prop where
+  | refl
+    {P : Proc} :
+    ------------
+    MPST P (ε) P
+
+  | stepR {l : Lbl} {ls : Lbls} {P P'' P' : Proc} :
+    (MPST P ls P'') → (P'' -[l]->ₚ P') →
+    ------------------------------------
+          MPST P (ls ∷ₗ l) P'
+
+notation:50 P " -[" ls "]->>ₚ " P' => MPST P ls P'
+
+------------------------- ENV-FUCNTION & TRANSITION RULES --------------------------
+
+def env {𝒢 : HyperEnv} {P : Proc} (_ : ⊢ P ∷ 𝒢) : HyperEnv := 𝒢
+
+inductive EnvStep : HyperEnv → Lbl → HyperEnv → Prop where
+  | one
+      {x : PName} :
+      EnvStep (x ∶ 1) (x⟦⟧) ∅
+
+  | tensor
+      {Γ Δ : Env} {x x' : PName} {A B : Types} :
+      EnvStep (Γ‚ Δ‚ x ∶ A ⊗ B) (x⟦x'⟧) (Γ‚ x'∶ A |ₕ Δ‚ x ∶ B)
+
+  | bot
+      {Γ : Env} {x : PName} :
+      EnvStep (Γ‚ x ∶ ⊥) (x⸨⸩) Γ
+
+  | parr
+      {Γ Δ : Env} {x x' : PName} {A B : Types} :
+      EnvStep (Γ‚ x ∶ A ⅋ B) (x⸨x'⸩) (Γ‚ x' ∶ A‚ Δ‚ x ∶ B)
+
+  | par₁
+      {𝒢 𝒢' ℋ : HyperEnv} {l : Lbl} :
+      EnvStep 𝒢 l 𝒢' →
+      -----------------------------
+      EnvStep (𝒢 |ₕ ℋ) l (𝒢' |ₕ ℋ)
+
+  | par₂
+      {𝒢 ℋ ℋ': HyperEnv} {l : Lbl} :
+      EnvStep ℋ l ℋ' →
+      -----------------------------
+      EnvStep (𝒢 |ₕ ℋ) l (𝒢 |ₕ ℋ')
+
+  | syn
+      {𝒢 𝒢' ℋ ℋ': HyperEnv} {l l' : Act} :
+      EnvStep 𝒢 l 𝒢' → EnvStep ℋ l' ℋ' →
+      ------------------------------------
+      EnvStep (𝒢 |ₕ ℋ) (l |ₗ l') (𝒢' |ₕ ℋ')
+
+  | one_bot
+      {𝒢 : HyperEnv} {Γ : Env} {x y : PName} :
+      EnvStep (𝒢 |ₕ x ∶ 1 |ₕ Γ‚ y ∶ ⊥) (x⟦⟧ |ₗ y⸨⸩) (𝒢 |ₕ Γ) →
+      ------------------------------------------------------
+      EnvStep (𝒢 |ₕ Γ) (τ) (𝒢 |ₕ Γ)
+
+  | tensor_parr
+      {𝒢 : HyperEnv} {Γ Δ Ξ : Env} {x x' y y': PName} {A B : Types} :
+      EnvStep
+        (𝒢 |ₕ Γ‚ Δ‚ x ∶ A ⊗ B |ₕ Ξ‚ y ∶ Aᗮ ⅋ Bᗮ)
+        (x⟦x'⟧ |ₗ y⸨y'⸩)
+        (𝒢 |ₕ Γ‚ x' ∶ A |ₕ Δ‚ x ∶ B |ₕ Ξ‚ y' ∶ Aᗮ‚ y ∶ Bᗮ) →
+      ---------------------------------------------------
+      EnvStep (𝒢 |ₕ Γ‚ Δ‚ Ξ) (τ) (𝒢 |ₕ Γ‚ Δ‚ Ξ)
+
+  | res
+      {𝒢 𝒢' : HyperEnv} {Γ Γ' Δ Δ' : Env} {x y : PName} {A B : Types} {l : Lbl} :
+      EnvStep (𝒢 |ₕ Γ‚ x ∶ Aᗮ |ₕ Δ‚ y ∶ A) (l) (𝒢' |ₕ Γ'‚ x ∶ Aᗮ |ₕ Δ'‚ y ∶ A) →
+      ----------------------------------------------------------------------------
+      EnvStep (𝒢 |ₕ Γ‚ Δ) l (𝒢' |ₕ Γ'‚ Δ')
+
+notation:50 P " -[" l "]->ₑ " P' => EnvStep P l P'
+
+inductive MEST : (𝒢 : HyperEnv) → Lbls → (𝒢' : HyperEnv) → Prop where
+  | refl
+    {𝒢 : HyperEnv} :
+    ------------
+    MEST 𝒢 (ε) 𝒢
+
+  | stepR {l : Lbl} {ls : Lbls} {𝒢 𝒢'' 𝒢' : HyperEnv} :
+    (MEST 𝒢 ls 𝒢'') → (𝒢'' -[l]->ₑ 𝒢') →
+    ----------------------------------
+          MEST 𝒢 (ls ∷ₗ l) 𝒢'
+
+notation:50 𝒢 " -[" ls "]->>ₑ " 𝒢' => MPST 𝒢 ls 𝒢'
